<?xml version="1.0" encoding="UTF-8"?>

<worksheet xmlns:xi="http://www.w3.org/2001/XInclude" margin="1in" bottom="1.25cm" solutions="yes" xml:id="ws_rings-review2" permid="Kdh">
    <title>Activity: Review of the Euclidean Algorithm</title>

    <introduction permid="kQD">
      <p permid="cgL">
        The goal of this activity is to remember how to use the Eulcidea Algorithm to find the greatest common divisor of two elements in a ring (numbers or polynomials, for us) and write the gcd as a linear combination of the two elements (which Bezout's lemma tells us we can do).
      </p>

      <example xml:id="example-integers-gcd" permid="EJu">
        <p permid="PSt">
          Let's find the gcd of <m>945</m> and <m>2415</m>.
          Repeatedly use the division algorithm:
          <md permid="Zmf">
            <mrow>2415 &amp; = 945 \cdot 2 + 525</mrow>
            <mrow>945 &amp; = 525 \cdot 1 + 420</mrow>
            <mrow>525 &amp; = 420 \cdot 1 + 105</mrow>
            <mrow>420 &amp; = 105 \cdot 4 + 0</mrow>
          </md>.
          Check: <m>105</m> divides all the quotients and remainders, and any other divisor of <m>945</m> and <m>2415</m> would also divide <m>105</m>.
          Therefore, <m>\gcd( 945, 2415 ) = 105</m>.
        </p>

        <p permid="vZC">
          Now work backwards to obtain numbers <m>r</m> and <m>s</m> such that <m>945 r + 2415 s = 105</m>.
          <md permid="Fto">
            <mrow>105 &amp; = 525 + (-1) \cdot 420</mrow>
            <mrow>&amp; = 525 + (-1) \cdot [945 + (-1) \cdot 525]</mrow>
            <mrow>&amp; = 2 \cdot 525 + (-1) \cdot 945</mrow>
            <mrow>&amp; = 2 \cdot [2415 + (-2) \cdot 945] + (-1) \cdot 945</mrow>
            <mrow>&amp; = 2 \cdot 2415 + (-5) \cdot 945</mrow>
          </md>.
          So <m>r = -5</m> and <m>s= 2</m>.
        </p>
      </example>
    </introduction>



<exercise workspace="15%" permid="QXM">
  <statement>
    <p permid="InU">
            Find the greatest common divisor of 471 and 564 using the Euclidean Algorithm and then find integers <m>r</m> and <m>s</m> such that <m>\gcd(471,564) = 471r+564s</m>. 
    </p>
  </statement>
  <solution permid="BOO">
    <p permid="mFQ">
            First we perform the Euclidean algorithm:
      <md permid="lAx">
        <mrow>564 = \amp 1\cdot 471 + 93 </mrow>
        <mrow>471 = \amp 5\cdot 93 + 6 </mrow>
        <mrow>93 = \amp 15\cdot 6 + 3 </mrow>
        <mrow>6 = \amp 2\cdot 3 + 0 </mrow>
      </md>
            so <m>\gcd(471,564) = 3</m>.
    </p>
    <p permid="SMZ">
            Now working backwards through the lines of the Euclidean algorithm to find <m>r</m> and <m>s</m>:
      <md permid="RHG">
        <mrow>3 = \amp 93 - 15\cdot 6</mrow>
        <mrow>3 = \amp 93 - 15\cdot (471 - 5\cdot 93) = -15\cdot 471 + 76\cdot 93</mrow>
        <mrow>3 =  \amp -15\cdot 471 + 76\cdot (564 - 471) = 76\cdot 564 - 91\cdot 471</mrow>
      </md>
            so <m>r = -91</m> and <m>s = 76</m>.
    </p>
  </solution>
</exercise>



<exercise workspace="15%" permid="xeV">
  <statement>
    <p permid="ovd">
            In the quotient ring <m>\Z/\langle 564 \rangle</m>, find an element <m>a + \langle 564\rangle</m> such that <m>(a+\langle 564\rangle)(471 + \langle 564\rangle) = 3 + \langle 564 \rangle</m>.  Explain why the previous question is helpful here.
    </p>
  </statement>
  <solution permid="hVX">
    <p permid="yUi">
            Using the work done in question 1 above, we need <m>a = -91</m>.
    </p>

    <p permid="fbr">
            Why is this?  Well we want <m>(a + \langle 564\rangle)(471 + \langle 564\rangle) = 3+\langle 564\rangle</m>.  In other words, we want <m>a\cdot 471 + \langle 564\rangle = 3 + \langle 564\rangle</m>, which is the same as asking that <m>3 \in a\cdot 471 + \langle 564\rangle</m>.  This is another way of requiring <me permid="teW">3 = a\cdot 471 + k\cdot 564</me>.  We found values of <m>a</m> and <m>k</m> to make this so above.
    </p>
  </solution>
</exercise>

<exercise workspace="1%" permid="dme">
  <statement>
    <p permid="UCm">
            Is <m>471 + \langle 564\rangle</m> a unit in <m>\Z/\langle 564\rangle</m>?  Explain.
    </p>
  </statement>
  <solution permid="Odg">
    <p permid="LiA">
            No.  Being a unit means that there is a multiplicative inverse.  That would be a coset <m>a + \langle 564 \rangle</m> that when multiplied by <m>471+\langle 564\rangle</m> gives the unity <m>1+\langle 564\rangle</m>.  We would then have <m>471a = 1 + 564k</m> for some <m>k \in \Z</m>.  But that would imply that <m>\gcd(471, 564) = 1</m>.
    </p>
  </solution>
</exercise>

<pagebreak />


<exercise workspace="28%" permid="Jtn">
  <statement>
    <p permid="AJv">
            In <m>\Q[x]</m>, find the gcd of the polynomials <m>a(x) = x^3 + 1</m> and <m>b(x) = x^4 + x^3 + 2x^2 + x - 1</m>.  Then express the gcd as a combination of the two polynomials (as in Bezout's lemma).
    </p>
  </statement>
  <solution permid="ukp">
    <p permid="rpJ">
            The gcd is <m>x+1</m>.  Working backwards we get <m>x+1 = \frac{1}{2}(x^2 + x + 2)a(x) - \frac{1}{2}x b(x)</m>.
    </p>
  </solution>
</exercise>

<exercise workspace="28%" permid="pAw">
  <statement>
    <p permid="gQE">
            Find the greatest common divisor of <m>x^{24}-1</m> and <m>x^{15}-1</m> in <m>\Q[x]</m>, and then express the gcd as a combination of the two polynomials.
    </p>
  </statement>
  <solution permid="ary">
    <p permid="XwS">
            Let's use the Euclidean algorithm:
      <md permid="xOP">
        <mrow>x^{24} - 1 =  \amp x^9(x^{15} - 1) + x^9 - 1 </mrow>
        <mrow>x^{15} - 1 =  \amp x^6(x^{9} - 1) + x^6 - 1 </mrow>
        <mrow>x^{9} - 1 =  \amp x^3(x^{6} - 1) + x^3 - 1 </mrow>
        <mrow>x^{6} - 1 =  \amp (x^3+1)(x^{3} - 1) + 0 </mrow>
      </md>
            Thus the gcd is <m>x^3-1</m>.
    </p>
    <p permid="DEb">
            Now work backwards:
      <md permid="dVY">
        <mrow>x^3 - 1 = \amp [x^9-1] - x^3[x^6-1] </mrow>
        <mrow>x^3 - 1 = \amp [x^9-1] - x^3([x^{15}-1] - x^6[x^9-1]) </mrow>
        <mrow> = \amp -x^3[x^{15}-1] + (x^9+1)[x^9-1] </mrow>
        <mrow>x^3 - 1 = \amp -x^3[x^{15}-1] + (x^9+1)([x^{24} - 1] - x^9[x^{15}-1] ) </mrow>
        <mrow> = \amp (x^9+1)[x^{24}-1] - (x^{18}+x^9 +x^3)[x^{15}-1]  </mrow>
      </md>
    </p>
  </solution>
</exercise>

<exercise workspace="20%" permid="VHF">
  <statement>
    <p permid="MXN">
            Find a coset <m>a(x) + \langle x^{24}-1\rangle</m> of <m>\Q[x]/\langle x^{24}-1\rangle</m> such that <m>(a(x) + \langle x^{24}-1\rangle)(x^{15}-1 + \langle x^{24}-1\rangle) = x^3-1 + \langle x^{24}-1\rangle</m>.
    </p>
  </statement>
  <solution permid="GyH">
    <p permid="jLk">
            Using the computations from the previous problem, we get <m>a(x) = -x^{18} - x^9 - x^3</m>.
    </p>
  </solution>
</exercise>

</worksheet>